add

formalization/DenotationCtx.v
@@ -30,3 +30,70 @@ Fixpoint ctxRst (Γ: listctx rty) (p: env -> Prop) :=
   end.
 
 Notation "'⟪' Γ '⟫' p " := (ctxRst Γ p) (at level 20, format "⟪ Γ ⟫ p", Γ constr).
+
+Lemma ctxRst_rewrite (Γ: listctx rty): forall (p1 p2: env -> Prop),
+    (forall Γv, p1 Γv -> p2 Γv) -> ctxRst Γ p1 -> ctxRst Γ p2.
+Admitted.
+
+Inductive ctxRstRev: listctx rty -> (env -> Prop) -> Prop :=
+| ctxRstRev_base: forall (p: env -> Prop), p ∅ -> ctxRstRev [] p
+| ctxRstRev_under: forall Γ (p: env -> Prop) (x: atom) b ϕ,
+  ctxRstRev Γ (fun Γv => exists (v: value), ⟦ [: b | m{Γv} ϕ] ⟧ v /\ p (<[x:=v]> Γv)) ->
+  ctxRstRev (Γ ++ [(x, [: b | ϕ])]) p
+| ctxRstRev_over: forall Γ (p: env -> Prop) (x: atom) b ϕ,
+  ctxRstRev Γ (fun Γv => forall (v: value), ⟦ {: b | m{Γv} ϕ} ⟧ v -> p (<[x:=v]> Γv)) ->
+  ctxRstRev (Γ ++ [(x, {: b | ϕ})]) p
+| ctxRstRev_arr: forall Γ (p: env -> Prop) (x: atom) τ1 τ2,
+    ctxRstRev Γ (fun Γv => forall (v: value), ⟦ m{Γv} (τ1 ⇨ τ2) ⟧ v -> p (<[x:=v]> Γv)) ->
+    ctxRstRev (Γ ++ [(x, τ1 ⇨ τ2)]) p.
+
+Global Hint Constructors ctxRstRev: core.
+
+Lemma ctxRstRev_rewrite (Γ: listctx rty): forall (p1 p2: env -> Prop),
+    (forall Γv, p1 Γv -> p2 Γv) -> ctxRstRev Γ p1 -> ctxRstRev Γ p2.
+Admitted.
+
+Lemma ctxRstRev_head_over (Γ: listctx rty): forall (p: env -> Prop) (x: atom) b ϕ,
+    (forall (v: value), ⟦ {: b | ϕ} ⟧ v -> (ctxRstRev (map (fun t => (t.1, substitute x v t.2)) Γ) (λ Γv : env, p (<[x:= v]> Γv)))) ->
+  ctxRstRev ((x, {:b|ϕ}) :: Γ) (λ Γv : env, p Γv).
+Proof.
+  induction Γ; intros.
+  - assert ([(x, {:b|ϕ})] = [] ++ [(x, {:b|ϕ})]) as Htmp. list_simplifier. auto.
+    rewrite Htmp. clear Htmp.
+    constructor. constructor. intros. apply H in H0. simpl in *. admit.
+  - 
+
+    simpl in H.
+  assert (forall Γv : env, ((fun Γv => forall v: value, (⟦{:b|ϕ}⟧) v → p (<[x := v]> Γv)) Γv) -> p Γv).
+  { intros. }
+  induction Γ; intros.
+  - apply ctxRstRev_over.
+
+Lemma CtxREq (Γ1 Γ2: listctx rty) (p: env -> Prop) :
+  ctxRst (Γ1 ++ Γ2) p -> ctxRst Γ1 (fun Γv1 => ctxRstRev Γ2 (fun Γv2 => p (Γv1 ∪ Γv2))).
+Proof.
+  generalize dependent Γ1.
+  induction Γ2; simpl; intros.
+  - listctx_set_simpl. eapply ctxRst_rewrite; eauto. intros.
+    constructor. rewrite map_union_empty; auto.
+  - apply IHΓ2.
+    assert (Γv ∪ ∅ = Γv). rewrite map_union_empty. auto. rewrite H1.  simplify_set_eq. naive_solver.
+
+    generalize dependent p.
+    assert (∀ Γv1 p, ctxRstRev [] (λ Γv2 : env, p (Γv1 ∪ Γv2)) = p Γv1). admit.
+    induction Γ1; simpl in *. intuition.
+    intros.
+    auto_destruct_pair. rename a into x. destruct r.
+    intros. apply H0 in H1. listctx_set_simpl.
+    + intros. rewrite H0.
+
+
+Lemma twoCtxREq (Γ: listctx rty) (p: env -> Prop) : ctxRst Γ p <-> ctxRstRev Γ p.
+Proof.
+  split.
+  - admit.
+  - induction Γ; simpl; intros. admit.
+    auto_destruct_pair. rename a into x. destruct r.
+    + intros.
+  - induction Γ; simpl; intros.
+
